Title: Systems of Linear Equations and GADate: 2025-07-03Category: MathSummary: The wedge product of GA can be used to derive Cramers rule, which is a formula that directly yields the solution to a linear system of equations.Author: Amir# Linear System of EquationsLinear systems of equations, or linear systems arise in the solution of a lot of real life applications in engineering and physics. In general, you can characterize them as multiple equations that are linear in each of their multiple variables. For example, a system of two linear equations in the variables $x$ and $y$ might look like$$    x + y = 1 \\    x - y = 1$$In this simple example the solution is given by$$    x = 1 \\    y = 0$$and it is unique, so there is no other pair $(x,y)$ that fulfills both of these linear equations simultaneously. In general, the problem of determining the number of solutions (or if those even exist at all) is dealt by the Rouché–Capelli theorem. But for now, we will mostly concern ourselves with linear systems of $n$ equations and $m$ variables, where $n=m$ since these are the most common type and they often admit unique solutions. Other linear systems are distinguished by if $n > m$, so there are more equations than variables, of if $n < m$, so there are less equations than variables. These linear systems are called overdetermined of underdetermined respectively.For our example system we had that $n = m = 2$. Often, a linear system is written in matrix form, so we can write it as a single equation with a matrix-vector product as$$    \begin{bmatrix}        1 & 1 \\        1 & -1    \end{bmatrix}    \begin{bmatrix}        x \\ y    \end{bmatrix}    =    \begin{bmatrix}        1 \\ 1    \end{bmatrix}$$Or, if we define new variables, we can write this as$$    A \mathbf{x} = \mathbf{b}.$$with$$    A = \begin{bmatrix}        1 & 1 \\        1 & -1    \end{bmatrix} \qquad    \mathbf{x} = \begin{bmatrix}        x \\ y    \end{bmatrix} \qquad    \mathbf{b} = \begin{bmatrix}        1 \\ 1    \end{bmatrix}.$$Although using a matrix is the standard approch, if we dont know much about matrices this tell us nothing new about solving the linear system. So, in order that we may use a different approch we instead interpret the linear system as the following linear span of vectors $\mathbf{a_1}$ and $\mathbf{a_2}$:$$    \mathbf{a_1} x + \mathbf{a_2} y = \mathbf{b}$$with$$    \mathbf{a_1} = \begin{bmatrix}        1 \\ 1    \end{bmatrix} \qquad    \mathbf{a_2} = \begin{bmatrix}        1 \\ -1    \end{bmatrix}$$This equation has the advantage that we do not mix matrices and vectors, but instead only scale the vectors with the scalar variables $x,y$ and add them up.# Wedge productAs a quick recap of the wedge product, we only need to know the following properties:The wedge product of two vectors $\mathbf{x},\mathbf{y}$ is anti-symmetric, so $$    \mathbf{x} \wedge \mathbf{y} = -\mathbf{y} \wedge \mathbf{x}.$$From this follows that the wedge product of a vector with itself always vanishes$$    \mathbf{x} \wedge \mathbf{x} = 0$$and in fact, that the wedge product of a vector with any other vector thats parallel to it also vanishes, since the latter can be seen as just a scaled version of the former.Therefore, using the wedge product we can eliminate vector terms from the linear system of equations, for this, take$$    \left( \mathbf{a_1} x + \mathbf{a_2} y \right) \wedge \mathbf{a_2} = \mathbf{b} \wedge \mathbf{a_2}$$and $$    \left( \mathbf{a_1} x + \mathbf{a_2} y \right) \wedge \mathbf{a_1} = \mathbf{b} \wedge \mathbf{a_1}.$$Distributing over the sums in parenthesis we get$$    \mathbf{a_1} \wedge \mathbf{a_2} x + \mathbf{a_2} \wedge \mathbf{a_2} y = \mathbf{b} \wedge \mathbf{a_2} \\    \mathbf{a_1} \wedge \mathbf{a_1} x + \mathbf{a_2} \wedge \mathbf{a_1} y = \mathbf{b} \wedge \mathbf{a_1}.$$Where we eliminate the vanishing terms $\mathbf{a_i} \wedge \mathbf{a_i}$ to get$$    \mathbf{a_1} \wedge \mathbf{a_2} x = \mathbf{b} \wedge \mathbf{a_2} \\    -\mathbf{a_1} \wedge \mathbf{a_2} y = \mathbf{b} \wedge \mathbf{a_1}.$$In the second equation I also flipped the vectors, which added a minus sign in order that both equations look more similar. After that, we only have to divide by $\mathbf{a_1} \wedge \mathbf{a_2}$ to solve for $x$ and $y$. This is possible using the geometric product, so in our example this bivector is equal to$$    \mathbf{a_1} \wedge \mathbf{a_2} = (e_1 + e_2) \wedge (e_1 - e_2) = -e_1 \wedge e_2 + e_2 \wedge e_1 = -2 e_1 \wedge e_2 = -2 e_{12}.$$And its right hand inverse is given by $$    (\mathbf{a_1} \wedge \mathbf{a_2})^{-1} = \frac{1}{2} e_{12},$$because $$    \frac{1}{2} e_{12} (-2 e_{12}) = -e_{12}^2 = 1.$$Note that the unit bivector $e_{12}$ squares to $-1$. Finally, the solution to the linear system is given by$$    x = \mathbf{b} \wedge \mathbf{a_2} (\mathbf{a_1} \wedge \mathbf{a_2})^{-1}\\    y = -\mathbf{b} \wedge \mathbf{a_1} (\mathbf{a_1} \wedge \mathbf{a_2})^{-1}.$$which we calculate to be$$    x = (e_1 + e_2) \wedge (e_1 - e_2) \frac{1}{2} e_{12} = -2 e_{12} \frac{1}{2} e_{12} = 1\\    y = (e_1 + e_2) \wedge (e_1 + e_2) \frac{1}{2} e_{12} = 0 \\$$# In Three Dimensions and UpOf course, this approach will also work in more dimensions. Given three equations of three variables the system looks like$$    \mathbf{a_1} x + \mathbf{a_2} y + \mathbf{a_3} z = \mathbf{b}$$So, we wedge from the right side with a bivector $\mathbf{a_i} \wedge \mathbf{a_j}$ in order to eliminate the two $\mathbf{a_i}$ and $\mathbf{a_j}$ at once, yielding three trivector equations$$    \mathbf{a_1} \wedge \mathbf{a_2} \wedge \mathbf{a_3} x = \mathbf{b} \wedge \mathbf{a_2} \wedge \mathbf{a_3} \\    \mathbf{a_2} \wedge \mathbf{a_3} \wedge \mathbf{a_1} y = \mathbf{b} \wedge \mathbf{a_3} \wedge \mathbf{a_1} \\    \mathbf{a_3} \wedge \mathbf{a_1} \wedge \mathbf{a_2} z = \mathbf{b} \wedge \mathbf{a_1} \wedge \mathbf{a_2} $$which can be solved for $x,y,z$ to give$$    x = \frac{\mathbf{b} \wedge \mathbf{a_2} \wedge \mathbf{a_3}}{\mathbf{a_1} \wedge \mathbf{a_2} \wedge \mathbf{a_3}} \\    y = \frac{ \mathbf{a_1} \wedge \mathbf{b} \wedge \mathbf{a_3} }{\mathbf{a_1} \wedge \mathbf{a_2} \wedge \mathbf{a_3}} \\    z = \frac{\mathbf{a_1} \wedge \mathbf{a_2} \wedge \mathbf{b}}{\mathbf{a_1} \wedge \mathbf{a_2} \wedge \mathbf{a_3}} .$$Notice that in this form, we can arrange the equations particularly symmetric without the use of a negative sign, can you see why?Generally, if we have even more variables $x_i$ where $1 \leq i \leq n$, this indicates that$$    x_i = \frac{\mathbf{a_1}\wedge ... \wedge \mathbf{a_{i-1}} \wedge \mathbf{b} \wedge \mathbf{a_{i+1}}... \wedge \mathbf{a_n}}{\mathbf{a_1}\wedge ... \wedge \mathbf{a_n}}.$$And remember, the $\mathbf{a_i}$ where the coefficients in front of of the variable $x_i$, so at index $i$ in the numerator we input the coefficients of $\mathbf{b}$ instead.This formula for solving linear systems is also known as Cramers rule, the only difference being that it is normally written in determinants instead of wedge products, because determinants are scalar valued, instead here we have quantities that are bivector, trivectors etc. but behave similarly and are also often invertible. Interestingly, we can now also see the reason why some linear systems do not have a unique solution. In this case, the multivector $\mathbf{a_1}\wedge ... \wedge \mathbf{a_n} = 0$ and so it is not invertible, because this wedge product can be interpreted as behaving like the (hyper)volume spanned by the vectors $\mathbf{a_i}$, this means that this volume collapses. The reason for this is, that one of the vectors $\mathbf{a_k}$ is contained in the span of all the other vectors $\mathbf{a_1}\wedge ... \wedge (\quad)_{k} \wedge  ... \wedge \mathbf{a_n}$ and so the total set of vectors is not linearly independent.